\documentclass[12pt]{exam}

\setlength{\topmargin}{-.75in} \addtolength{\textheight}{2.00in}
\setlength{\oddsidemargin}{.00in} \addtolength{\textwidth}{.25in}

\usepackage{amsmath,color,graphicx, multicol, nicefrac, enumerate}
\usepackage[inline]{asymptote}

\nofiles

\setlength{\parindent}{0in}

\pagestyle{plain}

\title{Differential equations exam 3 review - SP 17}
\author{Wray}
\begin{document}

\begin{asydef}
//
// Global Asymptote definitions can be put here.
//
usepackage("bm");
texpreamble("\def\V#1{\bm{#1}}");
\end{asydef}

\noindent {\sc {\bf {\Large Exam 3 review problems}}
            \hfill MAT 265, Spring 2017}
\newline
\newline
Solve the equation using the power series method.  Write out the first three nonzero terms of each linearly independent solution.

\begin{questions}

\question
$y^{\prime \prime} + x^2 y^{\prime} + x^2 y = 0$

\question
$y^{\prime \prime} + e^{-x} y = 0$

\end{questions}

Use the table to find the Laplace transform of each function.

\begin{questions}
\setcounter{question}{2}
\question
$f(t) = 3e^{6t}$

\question
$g(t) = 3 \cos t + \sin \left( 3t \right)$

\question
$h(t) = \left( t -1 \right)^2$

\question
$f(t) = e^{2t} \> \mathcal{U} \left( t - 3 \right)$

\question
$g(t) = \begin{cases}
	\cos 2t & \mbox{if } 0 \le t < 2\pi \\
    0 & \mbox{if } t \ge 2\pi
\end{cases}$

\question
$h(t) = \displaystyle \int_0^t e^{\tau} \> \sin \left( t - \tau \right) \> d\tau$
\smallskip
\newline
Do not evaluate the integral before finding the transform.

\question
$f(t)$ is the periodic function shown in the figure below.
\begin{center}
\begin{asy}
unitsize(x=0.75cm);
import graph;

xlimits( -1, 5);
ylimits( -2, 2);
xaxis(xmin=-1, xmax=5,Ticks("%"));
yaxis(ymin=-2, ymax=2, Ticks("%"));

labelx(2,2S+0.5W);
labelx(4,2S+0.5W);
labely(1,2W);
labely(-1,2W);
dot((0,-1));
dot((2,1));
draw((0,-1) -- (2,1));
dot((2,-1));
dot((4,1));
draw((2,-1) -- (4,1));
dot((4,-1));
draw((4,-1) -- (5.2,0.2));
draw(Label("$t$",position=Relative(1),align=2S),(currentpicture.userMin().x-1,0)--(currentpicture.userMax().x+1,0),Arrow);
draw(Label("$f(t)$",position=Relative(1),align=2W),(0,currentpicture.userMin().y-1)--(0,currentpicture.userMax().y+1),Arrow);

\end{asy}
\end{center}

\end{questions}

Find the inverse Laplace transform of each function.

\begin{questions}
\setcounter{question}{9}
\question
$F(s) = \dfrac{5}{s-6} - \dfrac{6s}{s^2+9}$

\question
$G(s) = \dfrac{s^2 + 9s +2}{(s-1)^2(s+3)}$

\question
$H(s) = \dfrac{3s + 2}{s^2 + 2s + 10}$

\question
$F(s) = \left( \dfrac{s+1}{s^2 + 4} \right) e^{-s}$

\end{questions}


\clearpage
SOLUTIONS

\begin{questions}
\question
$y(x) = c_0 \left( 1 - \dfrac{x^4}{12} + \dfrac{x^7}{126} + \ldots \right) +
    	c_1 \left( x - \dfrac{x^4}{12} - \dfrac{x^5}{20} + \ldots \right) $

\question
$y(x) = c_0 \left( 1 - \dfrac{x^2}{2} + \dfrac{x^3}{6} + \ldots \right) +
    	c_1 \left( x - \dfrac{x^3}{6} - \dfrac{x^4}{12} + \ldots \right) $

\question
$\dfrac{3}{s-6}$

\question
$\dfrac{3s}{s^2 + 1} + \dfrac{3}{s^2+9}$

\question
$\dfrac{s^2 - 2s + 2}{s^3}$

\question
$\dfrac{e^{-3(s-2)}}{s-2}$
\question
$\dfrac{s}{s^2+4} - \dfrac{e^{-2\pi s}}{s^2+4}$

\question
$\dfrac{1}{(s-1)(s^2+1)}$

\question
$\dfrac{1}{1 - e^{-2s}} \left( \dfrac{1}{s^2} - \dfrac{1}{s} - \dfrac{e^{-2s}}{s} - \dfrac{e^{-2s}}{s^2} \right)$

\question
$5e^{6t} - 6 \cos 3t$
\question
$2e^t + 3te^t - e^{-3t}$

\question
$3 e^{-t/2} \cos \left( \dfrac{\sqrt{39}}{2} t \right) + 
	\dfrac{1}{\sqrt{39}} e^{-t/2} \sin \left( \dfrac{\sqrt{39}}{2} t \right)$
 
\question
$\begin{cases}
0 & \mbox{if } t < 1 \\
\cos \left( 2t - 2 \right) + 
	\dfrac{1}{2} \sin \left( 2t - 2 \right) & \mbox{if } t \ge 1
\end{cases}$
\end{questions}
\end{document}